theories/examples/susp_correctness/helpers.v
@@ -3,7 +3,7 @@ From auth.rel_logic_tern_susp Require Export spec_rules spec_tactics.
 From auth.examples.susp_correctness Require Import resource_algebras definitions.
 
 Section authentikit_helpers.
-  Context `{!authG Σ, !seqG Σ, !visited_mapG Σ, !lg_mapG Σ, !mapG Σ, !capG Σ} (N : namespace).
+  Context `{!authG Σ, !seqG Σ, !visited_mapG Σ, !lg_mapG Σ, !mapG Σ, !capG Σ, !intransitG Σ} (N : namespace).
 
   Lemma sub_susp_count_update_map :
     ∀ t v c (id : nat) Nc m,
@@ -176,23 +176,25 @@ Section authentikit_helpers.
           assert (p = p') as <- by congruence.
           iDestruct "Hdisj" as "[Hpen|Hdone]".
           -- iMod (visited_transition_done m d γ id with "Hauth Hpending Hpen")
-               as "[Hauth' Hdone]"; [done|].
+               as "(Hauth' & Hdone)"; [done|].
              iDestruct (visit_done_keep with "Hdone") as "[Hdone #Hreached]".
              iModIntro.
-             iFrame "Hauth'".
-             iSplitL ""; [iApply "Hreached"|].
+             iSplitL "Hauth'"; [iExact "Hauth'"|].
+             iSplit; [iExact "Hreached"|].
              iSplitR "Hsusp"; [|iExact "Hsusp"].
              simpl.
              iExists (InjRV #susp). iSplit; [done|].
              iRight. iExists susp. iSplit; [done|].
              iRight. iExists p, γ.
              iFrame "Hlg' Hsusp_s Hfrag Hcap'". iSplit; [done|].
-             iRight. iExists id. iFrame "Hdone". iPureIntro. done.
-          -- iDestruct "Hdone" as (n) "[%Hn Hdone]".
-             by iDestruct (visited_invalid_1 with "[$Hpending $Hdone]") as %[].
+             iRight. iExists id. iSplit; [iPureIntro; done|].
+             iLeft. iExact "Hdone".
+          -- iDestruct "Hdone" as (n) "[%Hn [Hdone|[Hfin _]]]".
+             ++ by iDestruct (visited_invalid_1 with "[$Hpending $Hdone]") as %[].
+             ++ by iDestruct (visited_invalid_2 with "[$Hpending $Hfin]") as %[].
   Qed.
 
-  Lemma visited_update (id : nat) :
+  Lemma visited_update_done (id : nat) :
     ∀ t t' v (c pid Nc : nat) (susp : loc) (p : proph_id) γ m d,
       d !! γ = None →
       id > pid →
@@ -202,11 +204,103 @@ Section authentikit_helpers.
       susp ↦ᵥ{#3/4} InjLV (#pid, #p) -∗
       sub_susp_count_frags t v c pid Nc -∗
       visit_pending γ ==∗
-        visited_map_update_done m d γ id ∗ visit_reached_done γ id ∗
+        visit_reached_done γ id ∗
+        visited_map_update_done m d γ id ∗
         sub_susp_count_frags t v c pid Nc ∗
         susp ↦ᵥ{#3/4} InjLV (#pid, #p).
   Proof.
     iIntros (t t' v c pid Nc susp p γ m d Hfresh Hid Hsub)
+      "Hauth #Hlg Hsusp (#Hcap & %Hle & Hinner & Hagg) Hpending".
+    iAssert (∀ v_outer (tind : evi_type) (vind : val) (cind : nat) (tind' : evi_type),
+               ⌜sub_obj tind' vind (InjRV #susp)⌝ -∗
+               visited_mapg_auth m d -∗
+               lg_mapg_frag susp γ -∗
+               susp ↦ᵥ{#3/4} InjLV (#pid, #p) -∗
+               sub_susp_count tind vind cind pid Nc v_outer -∗
+               visit_pending γ ==∗
+               visit_reached_done γ id ∗
+               visited_map_update_done m d γ id ∗
+               sub_susp_count tind vind cind pid Nc v_outer ∗
+               susp ↦ᵥ{#3/4} InjLV (#pid, #p))%I
+      with "[]" as "Hlem".
+    { iClear "Hcap Hlg".
+      iIntros (v_outer t0).
+      iInduction t0 as [t1 t2 | t1 t2 | | | ] "IH".
+      all: iIntros (vind cind tind') "%Hsubind Hauth #Hlg Hsusp Hinner Hpending".
+      - (* tprod *)
+        simpl. iDestruct "Hinner" as (c1 c2 v1 v2 [-> <-]) "[Hc1 Hc2]".
+        destruct tind' as [t1' t2' | | | | ]; simpl in Hsubind; try done.
+        + destruct Hsubind as (v1' & v2' & Heq & Hdisj). injection Heq as <- <-.
+          destruct Hdisj as [<- | [<- | [Hsub1 | Hsub2]]].
+          * by iDestruct (sub_susp_count_ne_injr_loc with "Hc1") as %[].
+          * by iDestruct (sub_susp_count_ne_injr_loc with "Hc2") as %[].
+          * iMod ("IH" $! v1 c1 t1' Hsub1 with "Hauth Hlg Hsusp Hc1 Hpending")
+              as "(#Hreached & Hauth' & Hc1' & Hsusp')".
+            iModIntro. iFrame "Hreached Hauth' Hsusp'".
+            iExists c1, c2, v1, v2. by iFrame.
+          * iMod ("IH1" $! v2 c2 t2' Hsub2 with "Hauth Hlg Hsusp Hc2 Hpending")
+              as "(#Hreached & Hauth' & Hc2' & Hsusp')".
+            iModIntro. iFrame "Hreached Hauth' Hsusp'".
+            iExists c1, c2, v1, v2. by iFrame.
+        + destruct Hsubind as (? & [(Heq & _ & _) | (Heq & _ & _)]); discriminate.
+        + destruct Hsubind as (? & [Heq|Heq] & _); discriminate.
+      - (* tsum *)
+        simpl. iDestruct "Hinner" as "[Hl|Hr]".
+        + iDestruct "Hl" as (v1') "[-> Hc]".
+          destruct tind' as [t1' t2' | t1' t2' | | | ]; simpl in Hsubind; try done.
+          * destruct Hsubind as (? & ? & Heq & _); discriminate.
+          * destruct Hsubind as (v'' & [(Heq1 & _ & Heq3) | (Heq1 & _ & _)]).
+            -- subst v''. injection Heq1 as Heq. by apply no_fix_InjLV in Heq.
+            -- discriminate.
+          * destruct Hsubind as (? & [Heq|Heq] & _); discriminate.
+        + iDestruct "Hr" as (v2') "[-> Hc]".
+          destruct tind' as [t1' t2' | t1' t2' | | | ]; simpl in Hsubind; try done.
+          * destruct Hsubind as (? & ? & Heq & _); discriminate.
+          * destruct Hsubind as (v'' & [(Heq1 & _ & _) | (Heq1 & _ & Heq3)]).
+            -- discriminate.
+            -- subst v''. injection Heq1 as Heq. by apply no_fix_InjRV in Heq.
+          * destruct Hsubind as (v'' & [Heq|Heq] & Heqsv).
+            -- subst v''. injection Heq as ->.
+               by iDestruct (sub_susp_count_ne_injL_injR_susp with "Hc") as %[].
+            -- subst v''. injection Heq as ->.
+               iMod (sub_susp_count_eats_susp id _ cind pid Nc γ susp p v_outer m d
+                 with "Hauth Hlg Hsusp Hc Hpending")
+                 as "(Hauth' & #Hreached & Hc' & Hsusp')"; [done|done|].
+               iModIntro. iFrame "Hreached Hauth' Hsusp'".
+               iRight. iExists (InjRV (InjRV #susp)). by iFrame.
+      - (* tstring *)
+        simpl. iDestruct "Hinner" as "[Hv %Hc]". iDestruct "Hv" as (s) "->".
+        destruct tind'; simpl in Hsubind; try done.
+        + destruct Hsubind as (? & ? & Heq & _); discriminate.
+        + destruct Hsubind as (v'' & [(Heq & _) | (Heq & _)]); discriminate.
+        + destruct Hsubind as (? & [Heq|Heq] & _); discriminate.
+      - (* tint *)
+        simpl. iDestruct "Hinner" as "[Hv %Hc]". iDestruct "Hv" as (z) "->".
+        destruct tind'; simpl in Hsubind; try done.
+        + destruct Hsubind as (? & ? & Heq & _); discriminate.
+        + destruct Hsubind as (v'' & [(Heq & _) | (Heq & _)]); discriminate.
+        + destruct Hsubind as (? & [Heq|Heq] & _); discriminate.
+      - (* tauth *)
+        simpl. iDestruct "Hinner" as (v1) "[-> Hcases]".
+        destruct tind'; simpl in Hsubind; try done.
+        + destruct Hsubind as (? & ? & Heq & _); discriminate.
+        + destruct Hsubind as (? & [(Heq & _ & _) | (Heq & _ & Heq2)]).
+          * discriminate.
+          * subst. injection Heq as Heq. by apply no_fix_InjRV in Heq.
+        + destruct Hsubind as (? & [Heq|Heq] & ->).
+          * injection Heq as ->.
+            iDestruct "Hcases" as "[H|H]".
+            -- iDestruct "H" as (h) "%Heq'". destruct Heq' as [Heq' _]. discriminate.
+            -- iDestruct "H" as (susp') "[%Heq' _]". discriminate.
+          * injection Heq as ->.
+            iDestruct "Hcases" as "[H|H]".
+            -- iDestruct "H" as (h) "%Heq'". destruct Heq' as [Heq' _]. discriminate.
+            -- iDestruct "H" as (susp') "[%Heq' _]". by simplify_eq. }
+    iMod ("Hlem" $! v t v c t' Hsub with "Hauth Hlg Hsusp Hinner Hpending")
+      as "(#Hreached & Hauth' & Hinner & Hsusp)".
+    iModIntro. iFrame "Hreached Hauth' Hsusp Hcap Hinner Hagg". done.
+  Qed.
+    (* iIntros (t t' v c pid Nc susp p γ m d Hfresh Hid Hsub)
       "Hauth #Hlg Hsusp (#Hcap & %Hle & Hinner & Hagg) Hpending".
     iAssert (∀ v_outer (tind : evi_type) (vind : val) (cind : nat) (tind' : evi_type),
                ⌜sub_obj tind' vind (InjRV #susp)⌝ -∗
@@ -304,45 +398,190 @@ Section authentikit_helpers.
     iModIntro. iFrame "Hauth'".
     iSplitL ""; [iApply "Hreached"|].
     iFrame "Hsusp Hcap Hinner Hagg". done.
+  Qed. *)
+
+  Lemma sub_susp_count_finalizes_susp (id : nat) t (c pid Nc : nat) γ
+      (susp : loc) (p : proph_id) (v_outer : val) m d :
+    visited_mapg_auth m d -∗
+    lg_mapg_frag susp γ -∗
+    susp ↦ᵥ{#3/4} InjLV (#pid, #p) -∗
+    sub_susp_count t (InjRV (InjRV #susp)) c pid Nc v_outer -∗
+    visit_reached_done γ id -∗
+    intransit ==∗
+      visit_finished γ id ∗
+      visited_map_update_finished m d γ id ∗
+      sub_susp_count t (InjRV (InjRV #susp)) c pid Nc v_outer ∗
+      susp ↦ᵥ{#3/4} InjLV (#pid, #p).
+  Proof.
+    iIntros "Hauth #Hlg Hsusp Hcount #Hreached Hintr".
+    destruct t; simpl.
+    - iDestruct "Hcount" as (? ? ? ? [Heq _]) "_". discriminate.
+    - iDestruct "Hcount" as "[H|H]".
+      + iDestruct "H" as (?) "[%Heq _]". discriminate.
+      + iDestruct "H" as (v) "[%Heq H]". injection Heq as <-.
+        by iDestruct (sub_susp_count_ne_injr_loc with "H") as %[].
+    - iDestruct "Hcount" as "[Hv _]". iDestruct "Hv" as (?) "%Heq". discriminate.
+    - iDestruct "Hcount" as "[Hv _]". iDestruct "Hv" as (?) "%Heq". discriminate.
+    - (* tauth — substantive *)
+      iDestruct "Hcount" as (v1) "[%Heq Hcases]".
+      injection Heq as <-.
+      iDestruct "Hcases" as "[H|H]".
+      + iDestruct "H" as (h) "%Heq'". destruct Heq' as [Heq' _]. discriminate.
+      + iDestruct "H" as (susp') "[%Heq' Hinner]".
+        injection Heq' as Heq'. subst susp'.
+        iDestruct "Hinner" as "[Hfilled|Hsusp_inner]".
+        * iDestruct "Hfilled" as (h) "[Hsusp_f _]".
+          iDestruct (pointstoS_agree with "Hsusp Hsusp_f") as %[_ Heq''].
+          discriminate.
+        * iDestruct "Hsusp_inner" as (p' γ')
+            "(#Hlg' & Hsusp_s & %Hc & Hfrag & #Hcap' & Hdisj)".
+          iDestruct (lg_mapg_agree with "Hlg Hlg'") as "(<- & _ & _)".
+          iDestruct "Hdisj" as "[Hpen|Hinner_disj]".
+          { by iDestruct (visited_reached_done_invalid with "Hauth Hreached Hpen") as %[]. }
+          iDestruct "Hinner_disj" as (id' Hid') "[Hinner_done|[Hinner_fin Hintr2]]".
+          -- iDestruct (visit_done_keep with "Hinner_done") as "[Hinner_done #Hreached']".
+             iDestruct (visited_reached_done_agree with "Hreached Hreached'") as %->.
+             iMod (visited_transition_finished with "Hauth Hinner_done")
+               as "(Hauth' & #Hfin)".
+             iModIntro.
+             iSplit; [iExact "Hfin"|].
+             iSplitL "Hauth'"; [iExact "Hauth'"|].
+             iSplitR "Hsusp"; [|iExact "Hsusp"].
+             simpl.
+             iExists (InjRV #susp). iSplit; [done|].
+             iRight. iExists susp. iSplit; [done|].
+             iRight. iExists p', γ.
+             iFrame "Hlg' Hsusp_s Hfrag Hcap'". iSplit; [done|].
+             iRight. iExists id'. iSplit; [iPureIntro; done|].
+             iRight. iFrame "Hintr". iExact "Hfin".
+          -- by iDestruct (intransit_excl with "Hintr Hintr2") as %[].
   Qed.
 
-  (* When [c = 0] (all susps filled) and [Nc ≠ 0], the aggregator has
-     accumulated every [1/Nc] piece, giving the full fragment. *)
-  Lemma sub_susp_count_frags_terminated t v id Nc :
-    Nc ≠ 0 →
-    sub_susp_count_frags t v 0 id Nc -∗ mapg_frag #id 1 v.
-Proof. Admitted.
-    (* iIntros (HN) "(_ & %Hle & _ & Hagg)".
-    iDestruct "Hagg" as "[%Heq | [%Hlt Hq]]".
-    - lia.
-    - iDestruct "Hq" as (q Heqq) "Hfrag".
-      replace (Nc - 0) with Nc in Heqq by lia.
-      assert (q = 1%Qp) as ->; last done.
-      rewrite (Qp.mul_comm q) in Heqq.
-      apply (Qp.mul_inj_r (pos_to_Qp (Pos.of_nat Nc))).
-      rewrite Qp.mul_1_r. exact Heqq.
-  Qed. *)
+  Lemma visited_update_finished (id : nat) :
+      ∀ t t' v (c pid Nc : nat) (susp : loc) (p : proph_id) γ m d,
+        id > pid →
+        sub_obj t' v (InjRV #susp) →
+        visited_mapg_auth m d -∗
+        lg_mapg_frag susp γ -∗
+        susp ↦ᵥ{#3/4} InjLV (#pid, #p) -∗
+        sub_susp_count_frags t v c pid Nc -∗
+        visit_reached_done γ id ∗
+        intransit ==∗
+          visit_finished γ id ∗
+          visited_map_update_finished m d γ id ∗
+          sub_susp_count_frags t v c pid Nc ∗
+          susp ↦ᵥ{#3/4} InjLV (#pid, #p).
+  Proof.
+    iIntros (t t' v c pid Nc susp p γ m d Hid Hsub)
+      "Hauth #Hlg Hsusp (#Hcap & %Hle & Hinner & Hagg) [#Hreached Hintr]".
+    iAssert (∀ v_outer (tind : evi_type) (vind : val) (cind : nat) (tind' : evi_type),
+               ⌜sub_obj tind' vind (InjRV #susp)⌝ -∗
+               visited_mapg_auth m d -∗
+               lg_mapg_frag susp γ -∗
+               susp ↦ᵥ{#3/4} InjLV (#pid, #p) -∗
+               sub_susp_count tind vind cind pid Nc v_outer -∗
+               intransit ==∗
+               visit_finished γ id ∗
+               visited_map_update_finished m d γ id ∗
+               sub_susp_count tind vind cind pid Nc v_outer ∗
+               susp ↦ᵥ{#3/4} InjLV (#pid, #p))%I
+      with "[]" as "Hlem".
+    { iClear "Hcap Hlg".
+      iIntros (v_outer t0).
+      iInduction t0 as [t1 t2 | t1 t2 | | | ] "IH".
+      all: iIntros (vind cind tind') "%Hsubind Hauth #Hlg Hsusp Hinner Hintr".
+      - (* tprod *)
+        simpl. iDestruct "Hinner" as (c1 c2 v1 v2 [-> <-]) "[Hc1 Hc2]".
+        destruct tind' as [t1' t2' | | | | ]; simpl in Hsubind; try done.
+        + destruct Hsubind as (v1' & v2' & Heq & Hdisj). injection Heq as <- <-.
+          destruct Hdisj as [<- | [<- | [Hsub1 | Hsub2]]].
+          * by iDestruct (sub_susp_count_ne_injr_loc with "Hc1") as %[].
+          * by iDestruct (sub_susp_count_ne_injr_loc with "Hc2") as %[].
+          * iMod ("IH" $! v1 c1 t1' Hsub1 with "Hauth Hlg Hsusp Hc1 Hintr")
+              as "(#Hfin & Hauth' & Hc1' & Hsusp')".
+            iModIntro. iFrame "Hfin Hauth' Hsusp'".
+            iExists c1, c2, v1, v2. by iFrame.
+          * iMod ("IH1" $! v2 c2 t2' Hsub2 with "Hauth Hlg Hsusp Hc2 Hintr")
+              as "(#Hfin & Hauth' & Hc2' & Hsusp')".
+            iModIntro. iFrame "Hfin Hauth' Hsusp'".
+            iExists c1, c2, v1, v2. by iFrame.
+        + destruct Hsubind as (? & [(Heq & _ & _) | (Heq & _ & _)]); discriminate.
+        + destruct Hsubind as (? & [Heq|Heq] & _); discriminate.
+      - (* tsum *)
+        simpl. iDestruct "Hinner" as "[Hl|Hr]".
+        + iDestruct "Hl" as (v1') "[-> Hc]".
+          destruct tind' as [t1' t2' | t1' t2' | | | ]; simpl in Hsubind; try done.
+          * destruct Hsubind as (? & ? & Heq & _); discriminate.
+          * destruct Hsubind as (v'' & [(Heq1 & _ & Heq3) | (Heq1 & _ & _)]).
+            -- subst v''. injection Heq1 as Heq. by apply no_fix_InjLV in Heq.
+            -- discriminate.
+          * destruct Hsubind as (? & [Heq|Heq] & _); discriminate.
+        + iDestruct "Hr" as (v2') "[-> Hc]".
+          destruct tind' as [t1' t2' | t1' t2' | | | ]; simpl in Hsubind; try done.
+          * destruct Hsubind as (? & ? & Heq & _); discriminate.
+          * destruct Hsubind as (v'' & [(Heq1 & _ & _) | (Heq1 & _ & Heq3)]).
+            -- discriminate.
+            -- subst v''. injection Heq1 as Heq. by apply no_fix_InjRV in Heq.
+          * destruct Hsubind as (v'' & [Heq|Heq] & Heqsv).
+            -- subst v''. injection Heq as ->.
+               by iDestruct (sub_susp_count_ne_injL_injR_susp with "Hc") as %[].
+            -- subst v''. injection Heq as ->.
+               iMod (sub_susp_count_finalizes_susp id _ cind pid Nc γ susp p v_outer m d
+                 with "Hauth Hlg Hsusp Hc Hreached Hintr")
+                 as "(#Hfin & Hauth' & Hc' & Hsusp')".
+               iModIntro. iFrame "Hfin Hauth' Hsusp'".
+               iRight. iExists (InjRV (InjRV #susp)). by iFrame.
+      - (* tstring *)
+        simpl. iDestruct "Hinner" as "[Hv %Hc]". iDestruct "Hv" as (s) "->".
+        destruct tind'; simpl in Hsubind; try done.
+        + destruct Hsubind as (? & ? & Heq & _); discriminate.
+        + destruct Hsubind as (v'' & [(Heq & _) | (Heq & _)]); discriminate.
+        + destruct Hsubind as (? & [Heq|Heq] & _); discriminate.
+      - (* tint *)
+        simpl. iDestruct "Hinner" as "[Hv %Hc]". iDestruct "Hv" as (z) "->".
+        destruct tind'; simpl in Hsubind; try done.
+        + destruct Hsubind as (? & ? & Heq & _); discriminate.
+        + destruct Hsubind as (v'' & [(Heq & _) | (Heq & _)]); discriminate.
+        + destruct Hsubind as (? & [Heq|Heq] & _); discriminate.
+      - (* tauth *)
+        simpl. iDestruct "Hinner" as (v1) "[-> Hcases]".
+        destruct tind'; simpl in Hsubind; try done.
+        + destruct Hsubind as (? & ? & Heq & _); discriminate.
+        + destruct Hsubind as (? & [(Heq & _ & _) | (Heq & _ & Heq2)]).
+          * discriminate.
+          * subst. injection Heq as Heq. by apply no_fix_InjRV in Heq.
+        + destruct Hsubind as (? & [Heq|Heq] & ->).
+          * injection Heq as ->.
+            iDestruct "Hcases" as "[H|H]".
+            -- iDestruct "H" as (h) "%Heq'". destruct Heq' as [Heq' _]. discriminate.
+            -- iDestruct "H" as (susp') "[%Heq' _]". discriminate.
+          * injection Heq as ->.
+            iDestruct "Hcases" as "[H|H]".
+            -- iDestruct "H" as (h) "%Heq'". destruct Heq' as [Heq' _]. discriminate.
+            -- iDestruct "H" as (susp') "[%Heq' _]". by simplify_eq. }
+    iMod ("Hlem" $! v t v c t' Hsub with "Hauth Hlg Hsusp Hinner Hintr")
+      as "(#Hfin & Hauth' & Hinner & Hsusp)".
+    iModIntro. iFrame "Hfin Hauth' Hsusp Hcap Hinner Hagg". done.
+  Qed.
 
   (* Substantive tauth B2 update: reached via tsum's right branch when the
      external [susp] matches a B2 leaf. Consumes [c = 1] for the leaf,
      releases the [1/Nc] fragment, steps the verifier store. *)
-  Lemma count_update_eats_susp K tᵥ v' t (susp : loc) (c pid Nc : nat) (h : string) (v_outer : val) γ (n : nat) m d :
+  Lemma count_update_eats_susp K tᵥ v' t (susp : loc) (c pid Nc : nat) (h : string) (v_outer : val) γ (n : nat) :
     lg_mapg_frag susp γ -∗
-    visit_reached_done γ n -∗
-    visited_mapg_auth m d -∗
+    visit_finished γ n -∗
     sub_susp_count t (InjRV (InjRV #susp)) c pid Nc v_outer -∗
     susp ↦ᵥ{#(3/4)} InjLV (#pid, v') -∗
     spec_verifier tᵥ (fill K (#susp <- InjRV #h))
     ={⊤}=∗
       ⌜c = 1⌝ ∗
-      visited_map_update_finished m d γ n ∗
-      visit_finished γ n ∗
+      intransit ∗
       sub_susp_count t (InjRV (InjRV #susp)) (c-1) pid Nc v_outer ∗
       susp ↦ᵥ{#(3/4)} InjRV #h ∗
       spec_verifier tᵥ (fill K (#())) ∗
       mapg_frag #pid (1 / pos_to_Qp (Pos.of_nat Nc))%Qp v_outer.
   Proof.
-    iIntros "#Hlg #Hreached Hauth Hinner Hsusp Hspec".
+    iIntros "#Hlg #Hfin Hinner Hsusp Hspec".
     destruct t; simpl.
     - iDestruct "Hinner" as (? ? ? ? [Heq _]) "_". discriminate.
     - iDestruct "Hinner" as "[H|H]".
@@ -371,15 +610,13 @@ Proof. Admitted.
           iMod (step_verifier_store with "[$Hsusp_full $Hspec]") as "(Hspec & Hsusp_full)"; [done|].
           iEval (rewrite -Qp.three_quarter_quarter) in "Hsusp_full".
           iDestruct "Hsusp_full" as "[Hsusp Hsusp_s]".
-          iDestruct "Hdisj" as "[Hpending|Hdone]".
-          { by iDestruct (visited_reached_done_invalid with "Hauth Hreached Hpending") as %[]. }
-          iDestruct "Hdone" as (id Hidpid) "Hdone".
-          iDestruct (visit_done_keep with "Hdone") as "[Hdone #Hreached_id]".
-          iDestruct (visited_reached_done_agree with "Hreached Hreached_id") as %->.
-          iMod (visited_transition_finished with "Hauth Hdone") as "[Hauth_upd #Hfin]".
+          iDestruct "Hdisj" as "[Hpen|Hinner_disj]".
+          { by iDestruct (visited_invalid_2 with "[$Hpen $Hfin]") as %[]. }
+          iDestruct "Hinner_disj" as (id Hidpid) "[Hdone|[Hifin Hintr]]".
+          { by iDestruct (visited_invalid_3 with "[$Hdone $Hfin]") as %[]. }
           iModIntro.
           iSplitR; [done|].
-          iFrame "Hauth_upd Hfin".
+          iFrame "Hintr".
           iSplitR "Hsusp Hspec Hfrag".
           { iExists (InjRV #susp). iSplit; [done|].
             iRight. iExists susp. iSplit; [done|].
@@ -388,34 +625,28 @@ Proof. Admitted.
   Qed.
 
   Lemma count_update :
-    ∀ K tᵥ v v' (t t' : evi_type) (susp : loc) (c pid Nc : nat) (h : string) γ (n : nat) m d,
+    ∀ K tᵥ v v' (t t' : evi_type) (susp : loc) (c pid Nc : nat) (h : string) γ (n : nat),
       ⌜sub_obj t' v (InjRV #susp)⌝ -∗
       lg_mapg_frag susp γ -∗
-      visit_reached_done γ n -∗
-      visited_mapg_auth m d -∗
+      visit_finished γ n -∗
       sub_susp_count_frags t v c pid Nc -∗
       susp ↦ᵥ{#(3/4)} InjLV (#pid, v') -∗
       spec_verifier tᵥ (fill K (#susp <- InjRV #h))
       ={⊤}=∗
-        visited_map_update_finished m d γ n ∗
-        visit_finished γ n ∗
+        intransit ∗
         sub_susp_count_frags t v (c-1) pid Nc ∗
         susp ↦ᵥ{#(3/4)} InjRV #h ∗
         spec_verifier tᵥ (fill K (#())).
   Proof.
-    iIntros (K tᵥ v v' t t' susp c pid Nc h γ n m d)
-      "%Hsub #Hlg #Hreached Hauth (#Hcap & %Hle & Hinner & Hagg) Hsusp Hspec".
-    (* Run the inner structural induction to produce a fresh [1/Nc] fragment
-       and a decremented inner predicate. v_outer is threaded unchanged. *)
+    iIntros (K tᵥ v v' t t' susp c pid Nc h γ n)
+      "%Hsub #Hlg #Hfin (#Hcap & %Hle & Hinner & Hagg) Hsusp Hspec".
     iAssert (∀ v_outer (t : evi_type) (v : val) (c : nat) (t' : evi_type),
                ⌜sub_obj t' v (InjRV #susp)⌝ -∗
-               visited_mapg_auth m d -∗
                sub_susp_count t v c pid Nc v_outer -∗
                susp ↦ᵥ{#3/4} InjLV (#pid, v') -∗
                spec_verifier tᵥ (fill K (#susp <- InjRV #h)) ={⊤}=∗
                ⌜1 ≤ c⌝ ∗
-               visited_map_update_finished m d γ n ∗
-               visit_finished γ n ∗
+               intransit ∗
                sub_susp_count t v (c - 1) pid Nc v_outer ∗
                susp ↦ᵥ{#3/4} InjRV #h ∗
                spec_verifier tᵥ (fill K #()) ∗
@@ -424,7 +655,7 @@ Proof. Admitted.
     { iClear "Hcap".
       iIntros (v_outer tind).
       iInduction tind as [t1 t2 | t1 t2 | | | ] "IH".
-      all: iIntros (vind cind tind') "%Hsubind Hauth Hinner' Hsusp' Hspec'".
+      all: iIntros (vind cind tind') "%Hsubind Hinner' Hsusp' Hspec'".
       - (* tind = tprod *)
         simpl. iDestruct "Hinner'" as (c1 c2 v1 v2 [-> <-]) "[Hc1 Hc2]".
         destruct tind' as [t1' t2' | | | | ]; simpl in Hsubind; try done.
@@ -432,16 +663,16 @@ Proof. Admitted.
           destruct Hdisj as [<- | [<- | [Hsub1 | Hsub2]]].
           * by iDestruct (sub_susp_count_ne_injr_loc with "Hc1") as %[].
           * by iDestruct (sub_susp_count_ne_injr_loc with "Hc2") as %[].
-          * iMod ("IH" $! v1 c1 t1' Hsub1 with "Hauth Hc1 Hsusp' Hspec'")
-              as "(%Hc & Hauth' & #Hfin & Hc1' & Hsusp'' & Hspec'' & Hnew)".
+          * iMod ("IH" $! v1 c1 t1' Hsub1 with "Hc1 Hsusp' Hspec'")
+              as "(%Hc & Hintr & Hc1' & Hsusp'' & Hspec'' & Hnew)".
             iModIntro. iSplit; [iPureIntro; lia|].
-            iFrame "Hauth' Hfin Hsusp'' Hspec'' Hnew".
+            iFrame "Hintr Hsusp'' Hspec'' Hnew".
             iExists (c1 - 1), c2, v1, v2.
             iSplit; [iPureIntro; split; [done|lia]|]. iFrame.
-          * iMod ("IH1" $! v2 c2 t2' Hsub2 with "Hauth Hc2 Hsusp' Hspec'")
-              as "(%Hc & Hauth' & #Hfin & Hc2' & Hsusp'' & Hspec'' & Hnew)".
+          * iMod ("IH1" $! v2 c2 t2' Hsub2 with "Hc2 Hsusp' Hspec'")
+              as "(%Hc & Hintr & Hc2' & Hsusp'' & Hspec'' & Hnew)".
             iModIntro. iSplit; [iPureIntro; lia|].
-            iFrame "Hauth' Hfin Hsusp'' Hspec'' Hnew".
+            iFrame "Hintr Hsusp'' Hspec'' Hnew".
             iExists c1, (c2 - 1), v1, v2.
             iSplit; [iPureIntro; split; [done|lia]|]. iFrame.
         + destruct Hsubind as (v'' & [(Heq & _ & _) | (Heq & _ & _)]); discriminate.
@@ -465,10 +696,10 @@ Proof. Admitted.
             -- subst v''. injection Heq as ->.
                by iDestruct (sub_susp_count_ne_injL_injR_susp with "Hc") as %[].
             -- subst v''. injection Heq as ->.
-               iMod (count_update_eats_susp with "Hlg Hreached Hauth Hc Hsusp' Hspec'") as
-                 "(%Hc & Hauth' & #Hfin & Hc' & Hsusp'' & Hspec'' & Hnew)".
+               iMod (count_update_eats_susp with "Hlg Hfin Hc Hsusp' Hspec'") as
+                 "(%Hc & Hintr & Hc' & Hsusp'' & Hspec'' & Hnew)".
                iModIntro. iSplit; [iPureIntro; lia|].
-               iFrame "Hauth' Hfin Hsusp'' Hspec'' Hnew".
+               iFrame "Hintr Hsusp'' Hspec'' Hnew".
                iRight. iExists (InjRV (InjRV #susp)). by iFrame.
       - (* tind = tstring *)
         simpl. iDestruct "Hinner'" as "[Hv %Hc]". iDestruct "Hv" as (s) "->".
@@ -482,9 +713,7 @@ Proof. Admitted.
         + destruct Hsubind as (? & ? & Heq & _); discriminate.
         + destruct Hsubind as (v'' & [(Heq & _) | (Heq & _)]); discriminate.
         + destruct Hsubind as (v'' & [Heq|Heq] & _); discriminate.
-      - (* tind = tauth — sub_obj at tauth forces v to be SOMEV (InjL/InjR v')
-           with v' = InjRV #susp, which doesn't match any B1/B2 case (those
-           have v1 = InjRV #loc_literal). *)
+      - (* tind = tauth *)
         simpl. iDestruct "Hinner'" as (v1) "[-> Hcases]".
         destruct tind'; simpl in Hsubind; try done.
         + destruct Hsubind as (? & ? & Heq & _); discriminate.
@@ -500,15 +729,12 @@ Proof. Admitted.
             iDestruct "Hcases" as "[H|H]".
             -- iDestruct "H" as (h') "%Heq'". destruct Heq' as [Heq' _]. discriminate.
             -- iDestruct "H" as (susp') "[%Heq' _]". by simplify_eq. }
-    iMod ("Hlem" $! v t v c t' Hsub with "Hauth Hinner Hsusp Hspec")
-      as "(%Hc & Hauth' & #Hfin & Hinner & Hsusp & Hspec & Hnew)".
-    (* Combine the new [1/Nc] fragment with the existing aggregator. *)
-    iModIntro. iFrame "Hauth' Hfin Hsusp Hspec Hcap".
+    iMod ("Hlem" $! v t v c t' Hsub with "Hinner Hsusp Hspec")
+      as "(%Hc & Hintr & Hinner & Hsusp & Hspec & Hnew)".
+    iModIntro. iFrame "Hintr Hsusp Hspec Hcap".
     iSplit; [iPureIntro; lia|]. iFrame "Hinner".
-    (* Aggregator update: (Nc-c)/Nc + 1/Nc = (Nc-(c-1))/Nc. *)
     iDestruct "Hagg" as "[%HcN | [%HcN Hq]]".
-    - (* old aggregator empty (c = Nc); new has [1/Nc]. *)
-      iRight. iSplit; [iPureIntro; lia|].
+    - iRight. iSplit; [iPureIntro; lia|].
       iExists (1 / pos_to_Qp (Pos.of_nat Nc))%Qp. iFrame "Hnew". iPureIntro.
       rewrite Qp.mul_div_l.
       assert (Nc - (c - 1) = 1)%nat as -> by lia. done.
@@ -525,5 +751,117 @@ Proof. Admitted.
         rewrite pos_to_Qp_add. done.
       + iApply (mapg_frag_combine with "Hq Hnew").
   Qed.
+    (* iIntros (K tᵥ v v' t t' susp c pid Nc h γ n)
+      "%Hsub #Hlg #Hfin (#Hcap & %Hle & Hinner & Hagg) Hsusp Hspec".
+    iAssert (∀ v_outer (t : evi_type) (v : val) (c : nat) (t' : evi_type),
+               ⌜sub_obj t' v (InjRV #susp)⌝ -∗
+               sub_susp_count t v c pid Nc v_outer -∗
+               susp ↦ᵥ{#3/4} InjLV (#pid, v') -∗
+               spec_verifier tᵥ (fill K (#susp <- InjRV #h)) ={⊤}=∗
+               ⌜1 ≤ c⌝ ∗
+               sub_susp_count t v (c - 1) pid Nc v_outer ∗
+               susp ↦ᵥ{#3/4} InjRV #h ∗
+               spec_verifier tᵥ (fill K #()) ∗
+               mapg_frag #pid (1 / pos_to_Qp (Pos.of_nat Nc))%Qp v_outer)%I
+      with "[]" as "Hlem".
+    { iClear "Hcap".
+      iIntros (v_outer tind).
+      iInduction tind as [t1 t2 | t1 t2 | | | ] "IH".
+      all: iIntros (vind cind tind') "%Hsubind Hinner' Hsusp' Hspec'".
+      - (* tind = tprod *)
+        simpl. iDestruct "Hinner'" as (c1 c2 v1 v2 [-> <-]) "[Hc1 Hc2]".
+        destruct tind' as [t1' t2' | | | | ]; simpl in Hsubind; try done.
+        + destruct Hsubind as (v1' & v2' & Heq & Hdisj). injection Heq as <- <-.
+          destruct Hdisj as [<- | [<- | [Hsub1 | Hsub2]]].
+          * by iDestruct (sub_susp_count_ne_injr_loc with "Hc1") as %[].
+          * by iDestruct (sub_susp_count_ne_injr_loc with "Hc2") as %[].
+          * iMod ("IH" $! v1 c1 t1' Hsub1 with "Hc1 Hsusp' Hspec'")
+              as "(%Hc & Hc1' & Hsusp'' & Hspec'' & Hnew)".
+            iModIntro. iSplit; [iPureIntro; lia|].
+            iFrame "Hsusp'' Hspec'' Hnew".
+            iExists (c1 - 1), c2, v1, v2.
+            iSplit; [iPureIntro; split; [done|lia]|]. iFrame.
+          * iMod ("IH1" $! v2 c2 t2' Hsub2 with "Hc2 Hsusp' Hspec'")
+              as "(%Hc & Hc2' & Hsusp'' & Hspec'' & Hnew)".
+            iModIntro. iSplit; [iPureIntro; lia|].
+            iFrame "Hsusp'' Hspec'' Hnew".
+            iExists c1, (c2 - 1), v1, v2.
+            iSplit; [iPureIntro; split; [done|lia]|]. iFrame.
+        + destruct Hsubind as (v'' & [(Heq & _ & _) | (Heq & _ & _)]); discriminate.
+        + destruct Hsubind as (v'' & [Heq|Heq] & _); discriminate.
+      - (* tind = tsum *)
+        simpl. iDestruct "Hinner'" as "[Hl|Hr]".
+        + iDestruct "Hl" as (v1) "[-> Hc]".
+          destruct tind'; simpl in Hsubind; try done.
+          * destruct Hsubind as (? & ? & Heq & _); discriminate.
+          * destruct Hsubind as (v'' & [(Heq1 & _ & Heq2) | (Heq1 & _ & _)]).
+            -- subst v''. injection Heq1 as Heq. by apply no_fix_InjLV in Heq.
+            -- discriminate.
+          * destruct Hsubind as (v'' & [Heq|Heq] & _); discriminate.
+        + iDestruct "Hr" as (v2) "[-> Hc]".
+          destruct tind'; simpl in Hsubind; try done.
+          * destruct Hsubind as (? & ? & Heq & _); discriminate.
+          * destruct Hsubind as (v'' & [(Heq1 & _ & _) | (Heq1 & _ & Heq2)]).
+            -- discriminate.
+            -- subst v''. injection Heq1 as Heq. by apply no_fix_InjRV in Heq.
+          * destruct Hsubind as (v'' & [Heq|Heq] & Heqsv).
+            -- subst v''. injection Heq as ->.
+               by iDestruct (sub_susp_count_ne_injL_injR_susp with "Hc") as %[].
+            -- subst v''. injection Heq as ->.
+               iMod (count_update_eats_susp with "Hlg Hfin Hc Hsusp' Hspec'") as
+                 "(%Hc & Hc' & Hsusp'' & Hspec'' & Hnew)".
+               iModIntro. iSplit; [iPureIntro; lia|].
+               iFrame "Hsusp'' Hspec'' Hnew".
+               iRight. iExists (InjRV (InjRV #susp)). by iFrame.
+      - (* tind = tstring *)
+        simpl. iDestruct "Hinner'" as "[Hv %Hc]". iDestruct "Hv" as (s) "->".
+        destruct tind'; simpl in Hsubind; try done.
+        + destruct Hsubind as (? & ? & Heq & _); discriminate.
+        + destruct Hsubind as (v'' & [(Heq & _) | (Heq & _)]); discriminate.
+        + destruct Hsubind as (v'' & [Heq|Heq] & _); discriminate.
+      - (* tind = tint *)
+        simpl. iDestruct "Hinner'" as "[Hv %Hc]". iDestruct "Hv" as (z) "->".
+        destruct tind'; simpl in Hsubind; try done.
+        + destruct Hsubind as (? & ? & Heq & _); discriminate.
+        + destruct Hsubind as (v'' & [(Heq & _) | (Heq & _)]); discriminate.
+        + destruct Hsubind as (v'' & [Heq|Heq] & _); discriminate.
+      - (* tind = tauth *)
+        simpl. iDestruct "Hinner'" as (v1) "[-> Hcases]".
+        destruct tind'; simpl in Hsubind; try done.
+        + destruct Hsubind as (? & ? & Heq & _); discriminate.
+        + destruct Hsubind as (v'' & [(Heq & _ & _) | (Heq & _ & Heq2)]).
+          * discriminate.
+          * subst v''. injection Heq as Heq. by apply no_fix_InjRV in Heq.
+        + destruct Hsubind as (v'' & [Heq|Heq] & ->).
+          * injection Heq as ->.
+            iDestruct "Hcases" as "[H|H]".
+            -- iDestruct "H" as (h') "%Heq'". destruct Heq' as [Heq' _]. discriminate.
+            -- iDestruct "H" as (susp') "[%Heq' _]". discriminate.
+          * injection Heq as ->.
+            iDestruct "Hcases" as "[H|H]".
+            -- iDestruct "H" as (h') "%Heq'". destruct Heq' as [Heq' _]. discriminate.
+            -- iDestruct "H" as (susp') "[%Heq' _]". by simplify_eq. }
+    iMod ("Hlem" $! v t v c t' Hsub with "Hinner Hsusp Hspec")
+      as "(%Hc & Hinner & Hsusp & Hspec & Hnew)".
+    iModIntro. iFrame "Hsusp Hspec Hcap".
+    iSplit; [iPureIntro; lia|]. iFrame "Hinner".
+    iDestruct "Hagg" as "[%HcN | [%HcN Hq]]".
+    - iRight. iSplit; [iPureIntro; lia|].
+      iExists (1 / pos_to_Qp (Pos.of_nat Nc))%Qp. iFrame "Hnew". iPureIntro.
+      rewrite Qp.mul_div_l.
+      assert (Nc - (c - 1) = 1)%nat as -> by lia. done.
+    - iDestruct "Hq" as (q Heqq) "Hq".
+      iRight. iSplit; [iPureIntro; lia|].
+      iExists (q + 1 / pos_to_Qp (Pos.of_nat Nc))%Qp.
+      iSplit.
+      + iPureIntro.
+        rewrite Qp.mul_add_distr_r. rewrite Heqq.
+        rewrite Qp.mul_div_l.
+        assert (Nc - (c - 1) = (Nc - c) + 1)%nat as -> by lia.
+        assert (Nc - c ≠ 0)%nat as HNc by lia.
+        rewrite Nat2Pos.inj_add; [|lia|lia].
+        rewrite pos_to_Qp_add. done.
+      + iApply (mapg_frag_combine with "Hq Hnew").
+  Qed. *)
 
 End authentikit_helpers.
